Fixed the juicy_machine.v

concurrency/juicy_machine.v
@@ -639,7 +639,7 @@ Qed.
         intro H; inversion H.
     Qed.
     
-    Lemma juicyRestrictAccCoh': forall phi m (coh:access_cohere' m phi),
+    Lemma juicyRestrictAccCoh: forall phi m (coh:access_cohere' m phi),
         access_cohere (juicyRestrict coh) phi.
     Proof.
       unfold access_cohere; intros.
@@ -647,32 +647,54 @@ Qed.
       destruct ((perm_of_res (phi @ loc))) eqn:HH; try rewrite HH; simpl; reflexivity.
     Qed.
 
+    Lemma po_perm_of_res: forall r,
+       Mem.perm_order''  (perm_of_res' r) (perm_of_res r). 
+    Proof.
+      rewrite /perm_of_res /perm_of_res' => r.
+      destruct r; try solve[ apply po_refl].
+      assert (Mem.perm_order'' (perm_of_sh t0 (pshare_sh p)) (Some Nonempty)).
+      { destruct (perm_of_sh t0 (pshare_sh p)) eqn:HH; try solve[constructor].
+        apply perm_of_empty_inv in HH; destruct HH as [AA BB].
+        exfalso; apply (juicy_mem_ops.Abs.pshare_sh_bot _ BB). }
+      destruct k; first[ apply po_refl | assumption].
+    Qed.
+      
+      
     Lemma max_acc_coh_acc_coh: forall m phi,
         max_access_cohere m phi -> access_cohere' m phi.
     Proof.
       move=> m phi mac loc.
-      move: mac => /(_ loc).
-      rewrite /perm_of_res /perm_of_sh.
-      destruct (phi @ loc) eqn:HH.
-      destruct (eq_dec Share.bot Share.top) as [e|n]; [exfalso; apply Share.nontrivial; symmetry; assumption|].
-      
-      
-      - move: mac.
-    
-    Lemma juicyRestrictAccCoh: forall phi m (coh:max_access_cohere m phi),
-        access_cohere (juicyRestrict coh) phi.
+      move: mac => /(_ loc) mac.
+      eapply po_trans; eauto.
+      apply po_perm_of_res.
+    Qed.
+
+    Definition juicyRestrict':=
+      fun phi m macoh => @juicyRestrict phi m (max_acc_coh_acc_coh macoh).
+
+    Lemma juicyRestrictAccCoh': forall phi m (coh:max_access_cohere m phi),
+        access_cohere (juicyRestrict' coh) phi.
     Proof.
       unfold access_cohere; intros.
       rewrite juicyRestrictCurEq.
       destruct ((perm_of_res (phi @ loc))) eqn:HH; try rewrite HH; simpl; reflexivity.
     Qed.
 
+    Lemma po_join_sub': forall r1 r2 : resource,
+       join_sub r2 r1 ->
+       Mem.perm_order'' (perm_of_res' r1) (perm_of_res' r2).
+    Admitted.
+    
     Lemma mem_access_coh_sub: forall phi1 phi2 m,
           max_access_cohere m phi1 ->
           join_sub phi2 phi1 ->
           max_access_cohere m phi2.
     Proof.
-    Admitted.
+      rewrite /max_access_cohere => phi1 phi2 m H H0 loc.
+      eapply po_trans; eauto.
+      eapply po_join_sub'.
+      apply resource_at_join_sub; assumption.
+    Qed.
     
     Lemma mem_cohere_sub: forall phi1 phi2 m,
           mem_cohere' m phi1 ->
@@ -792,13 +814,8 @@ Admitted.
     
     (* PERSONAL MEM: Is the contents of the global memory, 
        with the juice of a single thread and the Cur that corresponds to that juice.*)
-    Definition personal_mem {m phi} (pr : mem_cohere' m phi) : juicy_mem.
-    Proof.
-      inversion pr.
-      eapply mkJuicyMem; eauto.
-      intros loc.
-      inversion pr; eauto.      eapply (juicyRestrictContentCoh (acc_coh0 pr) (cont_coh pr)).
-                                                                 
+    Definition acc_coh:= fun m phi pr => @max_acc_coh_acc_coh m phi (max_coh pr).
+    Definition personal_mem {m phi} (pr : mem_cohere' m phi) : juicy_mem:=
       mkJuicyMem
         (@juicyRestrict phi m (acc_coh pr))
         phi
@@ -1502,9 +1519,10 @@ Admitted.
       cut (Mem.perm_order'' (perm_of_res (allj @ (b,ofs))) (perm_of_res (r @ (b, ofs)))).
       {intros AA. eapply po_trans; eauto.
        inversion all_cohere0.
-       specialize (acc_coh0 (b, ofs)).
        rewrite getMaxPerm_correct.
-       apply acc_coh0. }
+       eapply max_acc_coh_acc_coh in max_coh0.
+       specialize (max_coh0 (b,ofs)).
+       apply max_coh0. }
       { apply po_join_sub.
         apply resource_at_join_sub. eapply compatible_lockRes_sub; eauto. }
     Qed.
@@ -1526,19 +1544,7 @@ Admitted.
       Lemma mem_cohere'_juicy_mem jm : mem_cohere' (m_dry jm) (m_phi jm).
       Proof.
         destruct jm as [m phi C A M L]; simpl.
-        constructor; auto; [].
-        intros loc; specialize (A loc); specialize (M loc).
-        destruct (phi @ loc).
-        * simpl in *.
-          unfold perm_of_sh in M.
-          if_tac in M.
-          -- exfalso; unshelve eapply (Share.nontrivial _); auto.
-          -- if_tac in M. now auto. congruence.
-        * simpl in *.
-          destruct k eqn:Ek.
-          now auto.
-          all: rewrite <- A.
-          all: now apply Mem.access_max.
+        constructor; auto.
       Qed.
       
       
@@ -1783,9 +1789,9 @@ Admitted.
       Lemma mem_cohere'_age m : hereditary age (mem_cohere' m).
       Proof.
         intros x y E.
-        intros [A B C D]; constructor.
+        intros [A B C]; constructor.
         - eapply contents_cohere_age; eauto.
-        - eapply access_cohere'_age; eauto.
+       (* - eapply access_cohere'_age; eauto.*)
         - eapply max_access_cohere_age; eauto.
         - eapply alloc_cohere_age; eauto.
       Qed.
